proof/invariant-abstract/ARM/ArchArch_AI.thy
@@ -40,11 +40,6 @@ lemma safe_parent_strg:
   done
 
 
-lemma asid_low_bits_pageBits:
-  "Suc (Suc asid_low_bits) = pageBits"
-  by (simp add: pageBits_def asid_low_bits_def)
-
-
 (* 32-bit instance of Detype_AI.range_cover_full *)
 lemma range_cover_full:
   "\<lbrakk>is_aligned ptr sz;sz<word_bits\<rbrakk> \<Longrightarrow> range_cover (ptr::word32) sz sz (Suc 0)"
